Fail at making a proper inductin principle

Translation/XTyping.v
@@ -191,6 +191,39 @@ Proof.
   intros Σ Γ t T H. induction H ; easy.
 Defined.
 
+Section ForallT2_size.
+
+  Context {A} (P : A -> A -> Type) (fn : forall x1 x2, P x1 x2 -> size).
+
+  Fixpoint forallt2_size {l1 l2 : list A} (f : ForallT2 P l1 l2) : size :=
+    match f with
+    | ForallT2_nil => 0
+    | ForallT2_cons x y l l' rxy rll' => (fn _ _ rxy + forallt2_size rll')%nat
+    end.
+
+End ForallT2_size.
+
+Definition typing_size {Σ Γ t T} (d : Σ ;;; Γ |-x t : T) : size.
+Proof.
+  revert Σ Γ t T d.
+  fix 5.
+  destruct 1 ;
+  repeat match goal with
+  | H : typing _ _ _ _ |- _ => apply typing_size in H
+  end ;
+  match goal with
+  | H : ForallT2 _ _ _ |- _ => idtac
+  | H1 : size, H2 : size, H3 : size |- _ => exact (S (Nat.max H1 (Nat.max H2 H3)))
+  | H1 : size, H2 : size |- _ => exact (S (Nat.max H1 H2))
+  | H1 : size |- _ => exact (S H1)
+  | _ : sdeclared_inductive _ _ _ _ |- _ => exact 2
+  | _ : sdeclared_constructor _ _ _ _ |- _ => exact 2
+  | _ => exact 1
+  end.
+  exact (S (Nat.max d1 (Nat.max d2
+     (forallt2_size _ (fun x y p => typing_size Σ Γ (snd x) (snd y) (snd p)) f)))).
+Defined.
+
 Scheme typing_ind' := Induction for typing Sort Type
   with wf_ind' := Induction for wf Sort Type
   with eq_term_ind' := Induction for eq_term Sort Type.
@@ -198,226 +231,228 @@ Scheme typing_ind' := Induction for typing Sort Type
 (* Combined Scheme typing_all from typing_ind , wf_ind , eq_term_ind. *)
 
 Definition typing_all : forall (Σ : sglobal_context)
-         (P0 : forall s : scontext, wf Σ s -> Type)
-         (P : forall (s : scontext) (s0 s1 : sterm),
-              Σ;;; s |-x s0 : s1 -> Type)
-         (P1 : forall (s : scontext) (s0 s1 s2 : sterm),
-               Σ;;; s |-x s0 = s1 : s2 -> Type),
-       P0 [] (wf_nil Σ) ->
+         (P0 : scontext -> Type)
+         (P : forall (s : scontext) (s0 s1 : sterm), Type)
+         (P1 : forall (s : scontext) (s0 s1 s2 : sterm), Type),
+       P0 [] ->
        (forall (Γ : scontext) (x : name) (A : sterm)
           (s : sort) (w : wf Σ Γ),
-        P0 Γ w ->
+        P0 Γ ->
         forall t : Σ;;; Γ |-x A : sSort s,
-        P Γ A (sSort s) t ->
-        P0 (Γ,, svass x A) (wf_snoc Σ Γ x A s w t))->
+        P Γ A (sSort s) ->
+        P0 (Γ,, svass x A)) ->
        (forall (Γ : scontext) (n : nat) (w : wf Σ Γ),
-        P0 Γ w ->
+        P0 Γ ->
         forall isdecl : n < #|Γ|,
         P Γ (sRel n)
           (lift0 (S n)
              (sdecl_type
-                (safe_nth Γ (exist (fun n0 : nat => n0 < #|Γ|) n isdecl))))
-          (type_Rel Σ Γ n w isdecl)) ->
+                (safe_nth Γ (exist (fun n0 : nat => n0 < #|Γ|) n isdecl))))) ->
        (forall (Γ : scontext) (s : sort) (w : wf Σ Γ),
-        P0 Γ w ->
-        P Γ (sSort s) (sSort (succ_sort s)) (type_Sort Σ Γ s w)) ->
+        P0 Γ ->
+        P Γ (sSort s) (sSort (succ_sort s))) ->
        (forall (Γ : scontext) (n : name) (t b : sterm)
           (s1 s2 : sort) (t0 : Σ;;; Γ |-x t : sSort s1),
-        P Γ t (sSort s1) t0 ->
+        P Γ t (sSort s1) ->
         forall t1 : Σ;;; Γ,, svass n t |-x b : sSort s2,
-        P (Γ,, svass n t) b (sSort s2) t1 ->
-        P Γ (sProd n t b) (sSort (max_sort s1 s2))
-          (type_Prod Σ Γ n t b s1 s2 t0 t1)) ->
+        P (Γ,, svass n t) b (sSort s2) ->
+        P Γ (sProd n t b) (sSort (max_sort s1 s2))) ->
        (forall (Γ : scontext) (n n' : name) (t b : sterm)
           (s1 s2 : sort) (bty : sterm) (t0 : Σ;;; Γ |-x t : sSort s1),
-        P Γ t (sSort s1) t0 ->
+        P Γ t (sSort s1) ->
         forall t1 : Σ;;; Γ,, svass n t |-x bty : sSort s2,
-        P (Γ,, svass n t) bty (sSort s2) t1 ->
+        P (Γ,, svass n t) bty (sSort s2) ->
         forall t2 : Σ;;; Γ,, svass n t |-x b : bty,
-        P (Γ,, svass n t) b bty t2 ->
-        P Γ (sLambda n t bty b) (sProd n' t bty)
-          (type_Lambda Σ Γ n n' t b s1 s2 bty t0 t1 t2)) ->
+        P (Γ,, svass n t) b bty ->
+        P Γ (sLambda n t bty b) (sProd n' t bty)) ->
        (forall (Γ : scontext) (n : name) (s1 s2 : sort)
           (t A B u : sterm) (t0 : Σ;;; Γ |-x A : sSort s1),
-        P Γ A (sSort s1) t0 ->
+        P Γ A (sSort s1) ->
         forall t1 : Σ;;; Γ,, svass n A |-x B : sSort s2,
-        P (Γ,, svass n A) B (sSort s2) t1 ->
+        P (Γ,, svass n A) B (sSort s2) ->
         forall t2 : Σ;;; Γ |-x t : sProd n A B,
-        P Γ t (sProd n A B) t2 ->
+        P Γ t (sProd n A B) ->
         forall t3 : Σ;;; Γ |-x u : A,
-        P Γ u A t3 ->
-        P Γ (sApp t n A B u) (B {0 := u})
-          (type_App Σ Γ n s1 s2 t A B u t0 t1 t2 t3)) ->
+        P Γ u A ->
+        P Γ (sApp t n A B u) (B {0 := u})) ->
        (forall (Γ : scontext) (s : sort) (A u v : sterm)
           (t : Σ;;; Γ |-x A : sSort s),
-        P Γ A (sSort s) t ->
+        P Γ A (sSort s) ->
         forall t0 : Σ;;; Γ |-x u : A,
-        P Γ u A t0 ->
+        P Γ u A ->
         forall t1 : Σ;;; Γ |-x v : A,
-        P Γ v A t1 ->
-        P Γ (sEq A u v) (sSort s) (type_Eq Σ Γ s A u v t t0 t1)) ->
+        P Γ v A ->
+        P Γ (sEq A u v) (sSort s)) ->
        (forall (Γ : scontext) (s : sort) (A u : sterm)
           (t : Σ;;; Γ |-x A : sSort s),
-        P Γ A (sSort s) t ->
+        P Γ A (sSort s) ->
         forall t0 : Σ;;; Γ |-x u : A,
-        P Γ u A t0 ->
-        P Γ (sRefl A u) (sEq A u u) (type_Refl Σ Γ s A u t t0)) ->
+        P Γ u A ->
+        P Γ (sRefl A u) (sEq A u u)) ->
        (forall (Γ : scontext) (ind : inductive) (w : wf Σ Γ),
-        P0 Γ w ->
+        P0 Γ ->
         forall univs decl (isdecl : sdeclared_inductive (fst Σ) ind univs decl),
-        P Γ (sInd ind) (decl.(sind_type)) (type_Ind Σ Γ ind w univs decl isdecl)) ->
+        P Γ (sInd ind) (decl.(sind_type))) ->
        (forall (Γ : scontext) (ind : inductive) (i : nat) (w : wf Σ Γ),
-        P0 Γ w ->
+        P0 Γ ->
         forall univs decl (isdecl : sdeclared_constructor (fst Σ) (ind, i) univs decl),
         P Γ (sConstruct ind i)
-          (stype_of_constructor (fst Σ) (ind, i) univs decl isdecl)
-          (type_Construct Σ Γ ind i w univs decl isdecl)) ->
+          (stype_of_constructor (fst Σ) (ind, i) univs decl isdecl)) ->
        (forall (Γ : scontext) (ind : inductive) (npar : nat) (p c : sterm) (brs : list (nat * sterm)) (args : list sterm)
           (decl : smutual_inductive_body) (isdecl : sdeclared_minductive (fst Σ) (inductive_mind ind) decl)
           (univs : universe_context) (decl' : sone_inductive_body) (isdecl' : sdeclared_inductive (fst Σ) ind univs decl')
           (e : sind_npars decl = npar),
         let pars := firstn npar args in
         forall (pty : sterm) (t : Σ;;; Γ |-x p : pty),
-        P Γ p pty t ->
+        P Γ p pty ->
         forall (indctx : scontext) (inds : sort) (pctx : scontext) (ps : sort) (btys : list (nat * sterm))
           (e0 : stypes_of_case pars p pty decl' = Some (indctx, inds, pctx, ps, btys))
           (e1 : scheck_correct_arity decl' ind indctx inds pars pctx = true)
           (t0 : Σ;;; Γ |-x c : Apps (sInd ind) indctx (sSort inds) args),
-        P Γ c (Apps (sInd ind) indctx (sSort inds) args) t0 ->
-        forall f8 : ForallT2 (fun x y : nat * sterm => (fst x = fst y) * (Σ;;; Γ |-x snd x : snd y)) brs btys,
-        P Γ (sCase (ind, npar) p c brs) (Apps p pctx (sSort ps) (skipn npar args ++ [c]))
-          (type_Case Σ Γ ind npar p c brs args decl isdecl univs decl' isdecl' e pty t indctx inds pctx ps btys e0 e1 t0 f8)) ->
+        P Γ c (Apps (sInd ind) indctx (sSort inds) args) ->
+        forall f8 : ForallT2 (fun x y : nat * sterm => (fst x = fst y) * (Σ;;; Γ |-x snd x : snd y) * P Γ (snd x) (snd y)) brs btys,
+        P Γ (sCase (ind, npar) p c brs) (Apps p pctx (sSort ps) (skipn npar args ++ [c]))) ->
        (forall (Γ : scontext) (t A B : sterm) (s : sort)
           (t0 : Σ;;; Γ |-x t : A),
-        P Γ t A t0 ->
+        P Γ t A ->
         forall t1 : Σ;;; Γ |-x B : sSort s,
-        P Γ B (sSort s) t1 ->
+        P Γ B (sSort s) ->
         forall e : Σ;;; Γ |-x A = B : sSort s,
-        P1 Γ A B (sSort s) e ->
-        P Γ t B (type_conv Σ Γ t A B s t0 t1 e)) ->
+        P1 Γ A B (sSort s) ->
+        P Γ t B) ->
        (forall (Γ : scontext) (u A : sterm) (t : Σ;;; Γ |-x u : A),
-        P Γ u A t -> P1 Γ u u A (eq_reflexivity Σ Γ u A t)) ->
+        P Γ u A -> P1 Γ u u A) ->
        (forall (Γ : scontext) (u v A : sterm) (e : Σ;;; Γ |-x u = v : A),
-        P1 Γ u v A e -> P1 Γ v u A (eq_symmetry Σ Γ u v A e)) ->
+        P1 Γ u v A -> P1 Γ v u A) ->
        (forall (Γ : scontext) (u v w A : sterm) (e : Σ;;; Γ |-x u = v : A),
-        P1 Γ u v A e ->
+        P1 Γ u v A ->
         forall e0 : Σ;;; Γ |-x v = w : A,
-        P1 Γ v w A e0 -> P1 Γ u w A (eq_transitivity Σ Γ u v w A e e0)) ->
+        P1 Γ v w A -> P1 Γ u w A) ->
        (forall (Γ : scontext) (s1 s2 : sort) (n : name)
           (A B t u : sterm) (t0 : Σ;;; Γ |-x A : sSort s1),
-        P Γ A (sSort s1) t0 ->
+        P Γ A (sSort s1) ->
         forall t1 : Σ;;; Γ,, svass n A |-x B : sSort s2,
-        P (Γ,, svass n A) B (sSort s2) t1 ->
+        P (Γ,, svass n A) B (sSort s2) ->
         forall t2 : Σ;;; Γ,, svass n A |-x t : B,
-        P (Γ,, svass n A) t B t2 ->
+        P (Γ,, svass n A) t B ->
         forall t3 : Σ;;; Γ |-x u : A,
-        P Γ u A t3 ->
+        P Γ u A ->
         P1 Γ (sApp (sLambda n A B t) n A B u) (t {0 := u})
-          (B {0 := u}) (eq_beta Σ Γ s1 s2 n A B t u t0 t1 t2 t3)) ->
+          (B {0 := u})) ->
        (forall (Γ : scontext) (s : sort) (T1 T2 t1 t2 : sterm)
           (e : Σ;;; Γ |-x t1 = t2 : T1),
-        P1 Γ t1 t2 T1 e ->
+        P1 Γ t1 t2 T1 ->
         forall e0 : Σ;;; Γ |-x T1 = T2 : sSort s,
-        P1 Γ T1 T2 (sSort s) e0 ->
-        P1 Γ t1 t2 T2 (eq_conv Σ Γ s T1 T2 t1 t2 e e0)) ->
+        P1 Γ T1 T2 (sSort s) ->
+        P1 Γ t1 t2 T2) ->
        (forall (Γ : scontext) (n1 n2 : name) (A1 A2 B1 B2 : sterm)
           (s1 s2 : sort) (e : Σ;;; Γ |-x A1 = A2 : sSort s1),
-        P1 Γ A1 A2 (sSort s1) e ->
+        P1 Γ A1 A2 (sSort s1) ->
         forall e0 : Σ;;; Γ,, svass n1 A1 |-x B1 = B2 : sSort s2,
-        P1 (Γ,, svass n1 A1) B1 B2 (sSort s2) e0 ->
+        P1 (Γ,, svass n1 A1) B1 B2 (sSort s2) ->
         forall t : Σ;;; Γ,, svass n1 A1 |-x B1 : sSort s2,
-        P (Γ,, svass n1 A1) B1 (sSort s2) t ->
+        P (Γ,, svass n1 A1) B1 (sSort s2) ->
         forall t0 : Σ;;; Γ,, svass n2 A2 |-x B2 : sSort s2,
-        P (Γ,, svass n2 A2) B2 (sSort s2) t0 ->
-        P1 Γ (sProd n1 A1 B1) (sProd n2 A2 B2) (sSort (max_sort s1 s2))
-          (cong_Prod Σ Γ n1 n2 A1 A2 B1 B2 s1 s2 e e0 t t0)) ->
+        P (Γ,, svass n2 A2) B2 (sSort s2) ->
+        P1 Γ (sProd n1 A1 B1) (sProd n2 A2 B2) (sSort (max_sort s1 s2))) ->
        (forall (Γ : scontext) (n1 n2 n' : name) (A1 A2 B1 B2 t1 t2 : sterm)
           (s1 s2 : sort) (e : Σ;;; Γ |-x A1 = A2 : sSort s1),
-        P1 Γ A1 A2 (sSort s1) e ->
+        P1 Γ A1 A2 (sSort s1) ->
         forall e0 : Σ;;; Γ,, svass n1 A1 |-x B1 = B2 : sSort s2,
-        P1 (Γ,, svass n1 A1) B1 B2 (sSort s2) e0 ->
+        P1 (Γ,, svass n1 A1) B1 B2 (sSort s2) ->
         forall e1 : Σ;;; Γ,, svass n1 A1 |-x t1 = t2 : B1,
-        P1 (Γ,, svass n1 A1) t1 t2 B1 e1 ->
+        P1 (Γ,, svass n1 A1) t1 t2 B1 ->
         forall t : Σ;;; Γ,, svass n1 A1 |-x B1 : sSort s2,
-        P (Γ,, svass n1 A1) B1 (sSort s2) t ->
+        P (Γ,, svass n1 A1) B1 (sSort s2) ->
         forall t0 : Σ;;; Γ,, svass n2 A2 |-x B2 : sSort s2,
-        P (Γ,, svass n2 A2) B2 (sSort s2) t0 ->
+        P (Γ,, svass n2 A2) B2 (sSort s2) ->
         forall t3 : Σ;;; Γ,, svass n1 A1 |-x t1 : B1,
-        P (Γ,, svass n1 A1) t1 B1 t3 ->
+        P (Γ,, svass n1 A1) t1 B1 ->
         forall t4 : Σ;;; Γ,, svass n2 A2 |-x t2 : B2,
-        P (Γ,, svass n2 A2) t2 B2 t4 ->
+        P (Γ,, svass n2 A2) t2 B2 ->
         P1 Γ (sLambda n1 A1 B1 t1) (sLambda n2 A2 B2 t2)
-          (sProd n' A1 B1)
-          (cong_Lambda Σ Γ n1 n2 n' A1 A2 B1 B2 t1 t2 s1 s2 e e0 e1 t
-             t0 t3 t4)) ->
+          (sProd n' A1 B1)) ->
        (forall (Γ : scontext) (n1 n2 : name) (s1 s2 : sort)
           (t1 t2 A1 A2 B1 B2 u1 u2 : sterm)
           (e : Σ;;; Γ |-x A1 = A2 : sSort s1),
-        P1 Γ A1 A2 (sSort s1) e ->
+        P1 Γ A1 A2 (sSort s1) ->
         forall e0 : Σ;;; Γ,, svass n1 A1 |-x B1 = B2 : sSort s2,
-        P1 (Γ,, svass n1 A1) B1 B2 (sSort s2) e0 ->
+        P1 (Γ,, svass n1 A1) B1 B2 (sSort s2) ->
         forall e1 : Σ;;; Γ |-x t1 = t2 : sProd n1 A1 B1,
-        P1 Γ t1 t2 (sProd n1 A1 B1) e1 ->
+        P1 Γ t1 t2 (sProd n1 A1 B1) ->
         forall e2 : Σ;;; Γ |-x u1 = u2 : A1,
-        P1 Γ u1 u2 A1 e2 ->
+        P1 Γ u1 u2 A1 ->
         forall t : Σ;;; Γ,, svass n1 A1 |-x B1 : sSort s2,
-        P (Γ,, svass n1 A1) B1 (sSort s2) t ->
+        P (Γ,, svass n1 A1) B1 (sSort s2) ->
         forall t0 : Σ;;; Γ,, svass n2 A2 |-x B2 : sSort s2,
-        P (Γ,, svass n2 A2) B2 (sSort s2) t0 ->
+        P (Γ,, svass n2 A2) B2 (sSort s2) ->
         forall t3 : Σ;;; Γ |-x t1 : sProd n1 A1 B1,
-        P Γ t1 (sProd n1 A1 B1) t3 ->
+        P Γ t1 (sProd n1 A1 B1) ->
         forall t4 : Σ;;; Γ |-x t2 : sProd n2 A2 B2,
-        P Γ t2 (sProd n2 A2 B2) t4 ->
+        P Γ t2 (sProd n2 A2 B2) ->
         forall t5 : Σ;;; Γ |-x u1 : A1,
-        P Γ u1 A1 t5 ->
+        P Γ u1 A1 ->
         forall t6 : Σ;;; Γ |-x u2 : A2,
-        P Γ u2 A2 t6 ->
+        P Γ u2 A2 ->
         P1 Γ (sApp t1 n1 A1 B1 u1) (sApp t2 n2 A2 B2 u2)
-          (B1 {0 := u1})
-          (cong_App Σ Γ n1 n2 s1 s2 t1 t2 A1 A2 B1 B2 u1 u2 e e0 e1 e2
-             t t0 t3 t4 t5 t6)) ->
+          (B1 {0 := u1})) ->
        (forall (Γ : scontext) (s : sort) (A1 A2 u1 u2 v1 v2 : sterm)
           (e : Σ;;; Γ |-x A1 = A2 : sSort s),
-        P1 Γ A1 A2 (sSort s) e ->
+        P1 Γ A1 A2 (sSort s) ->
         forall e0 : Σ;;; Γ |-x u1 = u2 : A1,
-        P1 Γ u1 u2 A1 e0 ->
+        P1 Γ u1 u2 A1 ->
         forall e1 : Σ;;; Γ |-x v1 = v2 : A1,
-        P1 Γ v1 v2 A1 e1 ->
-        P1 Γ (sEq A1 u1 v1) (sEq A2 u2 v2) (sSort s)
-          (cong_Eq Σ Γ s A1 A2 u1 u2 v1 v2 e e0 e1)) ->
+        P1 Γ v1 v2 A1 ->
+        P1 Γ (sEq A1 u1 v1) (sEq A2 u2 v2) (sSort s)) ->
        (forall (Γ : scontext) (s : sort) (A1 A2 u1 u2 : sterm)
           (e : Σ;;; Γ |-x A1 = A2 : sSort s),
-        P1 Γ A1 A2 (sSort s) e ->
+        P1 Γ A1 A2 (sSort s) ->
         forall e0 : Σ;;; Γ |-x u1 = u2 : A1,
-        P1 Γ u1 u2 A1 e0 ->
-        P1 Γ (sRefl A1 u1) (sRefl A2 u2) (sEq A1 u1 u1)
-          (cong_Refl Σ Γ s A1 A2 u1 u2 e e0)) ->
+        P1 Γ u1 u2 A1 ->
+        P1 Γ (sRefl A1 u1) (sRefl A2 u2) (sEq A1 u1 u1)) ->
        (forall (Γ : scontext) (ind : inductive) (npar : nat) (p p' c c' : sterm) (brs brs' : list (nat * sterm))
           (args : list sterm) (decl : smutual_inductive_body) (isdecl : sdeclared_minductive (fst Σ) (inductive_mind ind) decl)
           (univs : universe_context) (decl' : sone_inductive_body) (isdecl' : sdeclared_inductive (fst Σ) ind univs decl')
           (e : sind_npars decl = npar),
         let pars := firstn npar args in
         forall (pty : sterm) (e0 : Σ;;; Γ |-x p = p' : pty),
-        P1 Γ p p' pty e0 ->
+        P1 Γ p p' pty ->
         forall (indctx : scontext) (inds : sort) (pctx : scontext) (ps : sort) (btys : list (nat * sterm))
           (e1 : stypes_of_case pars p pty decl' = Some (indctx, inds, pctx, ps, btys))
           (e2 : scheck_correct_arity decl' ind indctx inds pars pctx = true)
           (e3 : Σ;;; Γ |-x c = c' : Apps (sInd ind) indctx (sSort inds) args),
-        P1 Γ c c' (Apps (sInd ind) indctx (sSort inds) args) e3 ->
+        P1 Γ c c' (Apps (sInd ind) indctx (sSort inds) args) ->
         forall
-          f9 : ForallT3 (fun x y z : nat * sterm => (fst x = fst y) * (fst y = fst z) * (Σ;;; Γ |-x snd x = snd y : snd z)) brs
+          f9 : ForallT3 (fun x y z : nat * sterm => (fst x = fst y) * (fst y = fst z) * (Σ;;; Γ |-x snd x = snd y : snd z) * P1 Γ (snd x) (snd y) (snd z)) brs
                  brs' btys,
-        P1 Γ (sCase (ind, npar) p c brs) (sCase (ind, npar) p' c' brs') (Apps p pctx (sSort ps) (skipn npar args ++ [c]))
-          (cong_Case Σ Γ ind npar p p' c c' brs brs' args decl isdecl univs decl' isdecl' e pty e0 indctx inds pctx ps btys e1 e2
-             e3 f9)) ->
+        P1 Γ (sCase (ind, npar) p c brs) (sCase (ind, npar) p' c' brs') (Apps p pctx (sSort ps) (skipn npar args ++ [c]))) ->
        (forall (Γ : scontext) (A u v e : sterm) (t : Σ;;; Γ |-x e : sEq A u v),
-        P Γ e (sEq A u v) t -> P1 Γ u v A (reflection Σ Γ A u v e t)) ->
-       (forall (s : scontext) (w : wf Σ s), P0 s w) *
+        P Γ e (sEq A u v) -> P1 Γ u v A) ->
+       (forall (s : scontext) (w : wf Σ s), P0 s) *
        (forall (s : scontext) (s0 s1 : sterm) (t : Σ;;; s |-x s0 : s1),
-           P s s0 s1 t) *
+           P s s0 s1) *
        (forall (s : scontext) (s0 s1 s2 : sterm) (e : Σ;;; s |-x s0 = s1 : s2),
-           P1 s s0 s1 s2 e).
+           P1 s s0 s1 s2).
 Proof.
-  intros; repeat split ; [
-  eapply wf_ind' | eapply typing_ind' | eapply eq_term_ind' ]; eauto.
-Defined.
+  intros.
+  repeat split ; [
+    eapply wf_ind' with (P0 := fun Γ _ => P0 Γ)
+                        (P := fun Γ t A _ => P Γ t A)
+                        (P1 := fun Γ t1 t2 A _ => P1 Γ t1 t2 A)
+  | eapply typing_ind' with (P0 := fun Γ _ => P0 Γ)
+                        (P := fun Γ t A _ => P Γ t A)
+                        (P1 := fun Γ t1 t2 A _ => P1 Γ t1 t2 A)
+  | eapply eq_term_ind' with (P0 := fun Γ _ => P0 Γ)
+                        (P := fun Γ t A _ => P Γ t A)
+                        (P1 := fun Γ t1 t2 A _ => P1 Γ t1 t2 A)
+  ] ; eauto.
+  - intros. eapply X10. all: try eassumption.
+    induction f.
+    + constructor.
+    + econstructor.
+      * destruct r.
+        repeat split ; try eassumption. admit.
+      * apply IHf.
+
+
+Abort.
